implement solver

theories/ContractEquations.v
@@ -7,6 +7,7 @@ Require Import Sorting.Sorted.
 Require Import Bool.Bool.
 Require Import Bool.Sumbool.
 Require Import List Setoid Permutation Sorted Orders.
+Require Import Coq.Arith.PeanoNat.
 Import ListNotations.
 
 Set Implicit Arguments.
@@ -373,3 +374,255 @@ intros. rewrite <- norm_c_eq. rewrite <- (norm_c_eq c1). unfold norm.
 apply comp_equiv_i_eq_sorted_monoms in H. rewrite H. apply c_refl.
 Qed.
 
+
+(**********Solver***********)
+
+Inductive Expr :=
+| Var : nat -> Expr
+| ESuccess : Expr
+| EFailure : Expr
+| EPlus : Expr -> Expr -> Expr
+| ESeq : Expr -> Expr -> Expr.
+
+
+Fixpoint contract_of_Expr vals e :=
+match e with
+| Var v => vals v
+| ESuccess => Success
+| EFailure => Failure
+| EPlus e0 e1 => (contract_of_Expr vals e0) _+_ (contract_of_Expr vals e1)
+| ESeq e0 e1 => (contract_of_Expr vals e0) _;_ (contract_of_Expr vals e1)
+end.
+
+Fixpoint monoms_of_Expr (e : Expr) : list (list nat) :=
+match e with
+| Var v => [[v]]
+| ESuccess => [[]]
+| EFailure => []
+| EPlus e0 e1 => (monoms_of_Expr e0) ++ (monoms_of_Expr e1)
+| ESeq e0 e1 => map (fun (a : list nat * list nat) => let (a1,a2):=a in a1++a2) (list_prod (monoms_of_Expr e0) (monoms_of_Expr e1))
+end.
+
+
+Definition list_contract_of_Expr_monoms (vals : nat -> Contract) (l : list (list nat)) := map (fun l0 => seq_fold (map vals l0)) l.
+
+
+
+
+
+Check forallb.
+Check Nat.eq_dec.
+Locate nat_dec.
+
+Definition inclb (l0 l1 : list (list nat)) :bool := forallb (fun a0 => existsb (fun a1 => if (list_eq_dec Nat.eq_dec) a0 a1 then true else false) l1) l0.
+
+Lemma inclb_iff : forall (l0 l1 : list (list nat)), inclb l0 l1 = true <-> incl l0 l1.
+Proof. unfold inclb. unfold incl. split. 
+- intros. rewrite forallb_forall in H. apply H in H0. rewrite existsb_exists in H0. destruct H0 as [x [P0 P1]].
+destruct (list_eq_dec Nat.eq_dec a x).
+  * subst. assumption.
+  * discriminate.
+- intros. rewrite forallb_forall. intros. apply H in H0. rewrite existsb_exists. exists x. split.
+  * assumption.
+  * destruct (list_eq_dec Nat.eq_dec x x).
+    ** reflexivity.
+    ** contradiction. 
+Qed.
+
+
+Lemma incl_reflect : forall (l0 l1 : list (list nat)), reflect (incl l0 l1) (inclb l0 l1).
+Proof. 
+intros. destruct (inclb l0 l1) eqn:Heqn.
+- constructor. rewrite inclb_iff in Heqn. assumption.
+- constructor. intro H. rewrite <- inclb_iff in H. rewrite Heqn in H. discriminate.
+Qed.
+
+Definition expr_eqb (e0 e1 : Expr) := inclb (monoms_of_Expr e0) (monoms_of_Expr e1) && inclb (monoms_of_Expr e1) (monoms_of_Expr e0).
+
+Definition expr_eq e0 e1 := incl (monoms_of_Expr e0) (monoms_of_Expr e1) /\ incl (monoms_of_Expr e1) (monoms_of_Expr e0).
+
+Lemma expr_eq_reflect : forall (e0 e1 : Expr), reflect (expr_eq e0 e1) (expr_eqb e0 e1).
+Proof.
+intros. unfold expr_eq. unfold expr_eqb. destruct ((inclb (monoms_of_Expr e0) (monoms_of_Expr e1) &&
+   inclb (monoms_of_Expr e1) (monoms_of_Expr e0))) eqn:Heqn. 
+- apply andb_prop in Heqn as [H0 H1]. constructor. rewrite inclb_iff in H0.
+  rewrite inclb_iff in H1. split ; auto.
+- destruct (incl_reflect ((monoms_of_Expr e0)) (monoms_of_Expr e1)).
+  * simpl in Heqn. constructor. intros [H3 H4]. rewrite <- inclb_iff in H4. rewrite Heqn in H4. discriminate.
+  * constructor. intros [H0 H1]. contradiction.
+Qed.
+
+
+
+Lemma expr_monoms : forall (e : Expr)(vals : nat -> Contract), contract_of_Expr vals e =R= plus_fold (map (fun l => seq_fold (map vals l)) (monoms_of_Expr e)).
+Proof.
+induction e;intros.
+- simpl. auto. rewrite c_plus_neut. auto.
+- simpl. auto.
+- simpl. auto.
+- simpl. apply c_eq_completeness. intros. rewrite map_app. rewrite plus_fold_app.
+  apply c_eq_soundness. auto.
+- simpl. rewrite map_map. apply c_eq_completeness. intros. rewrite in_plus_fold. split.
+  * intros. inversion H. subst. specialize IHe1 with vals.
+    specialize IHe2 with vals. eapply c_eq_soundness in IHe1.
+    rewrite in_plus_fold in IHe1. eapply IHe1 in H3. 
+    eapply c_eq_soundness in IHe2. rewrite in_plus_fold in IHe2. 
+    eapply IHe2 in H4. destruct H3 as [c3 [P31 P32]].
+    destruct H4 as [c4 [P41 P42]]. rewrite in_map_iff in P31. 
+    rewrite in_map_iff in P41. destruct P31 as [l1 [P31 P31']].
+    destruct P41 as [l2 [P41 P41']]. exists (seq_fold (map vals (l1++l2))).
+    split.
+    ** rewrite in_map_iff. exists (l1,l2). split.
+      *** reflexivity.
+      *** rewrite in_prod_iff. split ; auto.
+    ** rewrite map_app. rewrite seq_fold_app. subst. constructor; auto.
+  * intros. destruct H as [c [P1 P2]]. rewrite in_map_iff in P1.
+    destruct P1 as [p [P1 P1']]. destruct p. rewrite map_app in P1.
+    specialize IHe1 with vals. specialize IHe2 with vals. 
+    pose proof (c_seq_morph IHe1 IHe2). apply c_eq_soundness with (s:=s) in H.
+    rewrite H. subst. rewrite seq_fold_app in P2. inversion P2.
+    constructor. apply in_plus_fold. exists (seq_fold (map vals l)).
+    apply in_prod_iff in P1' as [P1' P2']. split.
+    ** rewrite in_map_iff. exists l. split. reflexivity. assumption.
+    ** assumption.
+    **     apply in_prod_iff in P1' as [P1' P2']. apply in_plus_fold. exists (seq_fold (map vals l0)). split. 
+      *** rewrite in_map_iff. exists l0.  split. reflexivity. assumption.
+      *** assumption.
+Qed.
+
+Lemma c_eqP : forall (e0 e1 : Expr)(vals : nat -> Contract), expr_eqb e0 e1 = true -> (contract_of_Expr vals e0) =R= (contract_of_Expr vals e1).
+Proof.
+intros. repeat rewrite expr_monoms. apply c_eq_completeness. intros. repeat rewrite in_plus_fold. 
+destruct (expr_eq_reflect e0 e1).
+- unfold expr_eq in e. destruct e. split;intros.
+  * destruct H2 as [x [P1 P2]]. apply in_map_iff in P1 as [l [Pl1 Pl2]].
+    unfold incl in H0. exists x. split. rewrite in_map_iff. exists l. split ; auto. assumption.
+  * destruct H2 as [x [P1 P2]]. apply in_map_iff in P1 as [l [Pl1 Pl2]].
+    unfold incl in H0. exists x. split. rewrite in_map_iff. exists l. split ; auto. assumption.
+- discriminate.
+Qed.
+
+
+Definition ex_con := Transfer _._ Notify _._ Success _+_ Notify _._ Success.
+
+Definition my_vals n :=
+if Nat.eq_dec 0 n then (Event Transfer) else if Nat.eq_dec 1 n then (Event Notify) else Failure.
+
+Definition expr1 := (EPlus (ESeq (Var 0) (ESeq (Var 1) ESuccess)) (ESeq (Var 1) ESuccess)).
+
+Definition expr2 := (EPlus (ESeq (Var 1) ESuccess) (ESeq (Var 0) (ESeq (Var 1) ESuccess))).
+
+Eval compute in (contract_of_Expr my_vals expr1).
+Eval compute in (contract_of_Expr my_vals expr2).
+
+Lemma test : (Transfer _._ Notify _._ Success _+_ Notify _._ Success) =R= 
+             (Notify _._ Success _+_ Transfer _._ Notify _._ Success ).
+Proof.
+exact (@c_eqP expr1 expr2 my_vals eq_refl).
+Qed.
+
+Ltac intern vars e :=
+  let rec loop n vars' :=
+    match vars' with
+    | [] =>
+      let vars'' := eval simpl in (rev (e::(rev vars))) in
+      constr:((n, vars''))
+    | e :: ?vars'' => constr:((n, vars))
+    | _ :: ?vars'' => loop (S n) vars''
+    end in
+  loop 0 vars.
+
+Ltac reify_expr vars c :=
+  match c with
+  | ?c1 _+_ ?c2 =>
+    let r1 := reify_expr vars c1 in
+    match r1 with
+    | (?qe1, ?vars') =>
+      let r2 := reify_expr vars' c2 in
+      match r2 with
+      | (?qe2, ?vars'') => constr:((EPlus qe1 qe2, vars''))
+      end
+    end
+  | ?c1 _;_ ?c2 =>
+    let r1 := reify_expr vars c1 in
+    match r1 with
+    | (?qe1, ?vars') =>
+      let r2 := reify_expr vars' c2 in
+      match r2 with
+      | (?qe2, ?vars'') => constr:((ESeq qe1 qe2, vars''))
+      end
+    end
+  | _ =>
+    let r := intern vars c in
+    match r with
+    | (?n, ?vars') => constr:((Var n, vars'))
+    end
+  end.
+
+Check nth 0.
+
+
+
+Fixpoint fun_of_list_aux (l : list  (nat * Contract)) :=
+match l with
+| [] => (fun  _ => Failure)
+| (n,c)::l' => let f2 := fun_of_list_aux l'
+               in (fun t => if Nat.eq_dec n t then c else f2 t)
+end.
+
+Definition fun_of_list l := fun_of_list_aux (combine (seq 0 (length l)) l).
+
+Definition fun_test := fun_of_list [Failure;Success].
+
+Ltac csl_solve :=
+  match goal with
+  | |- ?c1 =R= ?c2 =>
+    let r1 := reify_expr (@nil Contract) c1 in
+    match r1 with
+    | (?qe1, ?vm') =>
+      let r2 := reify_expr vm' c2 in
+      match r2 with
+      | (?qe2, ?vm'') => exact (@c_eqP qe1 qe2 (fun_of_list vm'') eq_refl) 
+      end
+    end
+  end.
+
+
+Lemma test2 : forall c0 c0' c1 c1', (c0 _+_ c1) _;_ (c0' _+_ c1') =R= c0 _;_ c0' _+_ c0 _;_ c1' _+_ c1 _;_ c0' _+_ c1 _;_ c1'. 
+Proof.
+intros.
+ csl_solve.
+Qed.
+
+
+
+
+
+
+
+
+
+
+
+
+
+
+
+
+
+
+
+
+
+
+
+
+
+
+
+
+
+
+
+
+ 
